# Problem Set 11

## 1. Partial Equilibrium

$$
\begin{cases}
u=m+\ln x & \text{utility of a single consumer} \\
\omega=1 & \text{endowment of numeraire} \\
N & \text{number of firms} \\
x & \text{quantity of goods procuced by $N$ firms} \\
z_j & \text{amount of numeraire used by firm $j$ in the production} \\
q_j=\sqrt{z_j} & \text{technology} \\
p & \text{price of the consumption goods}
\end{cases}
$$

* **Consumer problem:**
  $$
  \begin{align}
  \max_{m,x} & \quad m+\ln x \\
  \textrm{s.t.} & \quad m+p\cdot x\leq 1\cdot\omega+p\cdot0+\Pi
  \end{align}
  $$
  Constraint must hold with equality due to monotone preference
  $$
  \max_{x\geq0}\quad 1+\Pi-p\cdot x+\ln x
  $$

  $$
  \text{FOC:}\quad-p+\frac{1}{x}=0\implies x=\frac{1}{p}\quad\text{demand is independent of wealth}
  $$

* **Firm problem:**
  $$
  \text{Cost of producing quantity $q_j$:}\quad c(q)=q_j^2
  $$
  
  $$
  \Pi=N\cdot(p\cdot q_j-q_j^2)
  $$
  
  $$
  \max_{q_j}\quad p\cdot q_j-q_j^2
  $$
  
  $$
  \text{FOC:}\quad p-2q_j=0\implies q_j=\frac{p}{2}
  $$
  
* **Market clearing:**
  $$
  \text{Aggregate production:}\quad q=\sum_{j=1}^{N}q_j=\sum_{j=1}^{N}\frac{p}{2}=N\cdot\frac{p}{2}
  $$

  $$
  \begin{align}
  \text{demand}&=\text{supply} \\
  x&=q \\
  \frac{1}{p}&=N\cdot\frac{p}{2} \\
  p^*&=\sqrt{\frac{2}{N}}
  \end{align}
  $$

  $$
  \begin{align}
  x^*&=\frac{1}{p^*}=\sqrt{\frac{N}{2}} \\
  q_j^*&=\frac{p^*}{2}=\frac{1}{\sqrt{2N}} \\
  z_j^*&=(q_j^*)^2=\frac{1}{2N} \\
  \Pi^*&=N\cdot(p^*\cdot q_j^*-(q_j^*)^2)=
  N\left(\sqrt{\frac{2}{N}}\cdot\frac{1}{\sqrt{2N}}-\frac{1}{2N}\right)=\frac{1}{2} \\
  m^*&=\Pi^*+\omega-p^*\cdot x^*=\frac{1}{2}+1-\sqrt{\frac{2}{N}}\cdot\sqrt{\frac{N}{2}}=\frac{1}{2}
  \end{align}
  $$



## 2. Partial Equilibrium: Pareto Set

* There are $I=2$ consumers with utility $u_i=m_i+\phi_1(x)$ , where $\phi_i'>0$ and $\phi_i''<0$ .
* $J=1$ firm uses the numeraire good to produce output $y_i$ with cost function $c_j(y_j)\geq0$ , where $c_j'c_j''>0$ . 
* $c_j(y_j)$ corresponds to the quantity of input used by firm $j$ to produce $y_j\geq0$ units of output.
* The aggregate endowment of the production good (numeraire) is $\omega>0$ .

### 2(a)

$$
\begin{align}
\max_{m_1,x_1,m_2,x_2} \quad & m_1+\phi_1(x_1) \\
\textrm{s.t.} \quad & 
\begin{cases}
m_2+\phi_2(x_2)\geq u_2 & (\lambda)\\
x_1+x_2\leq y_j & (\mu) \\
m_1+m_2+c_j(y_j)\leq\omega & (\eta)
\end{cases}
\end{align}
$$

$$
\mathcal{L}=m_1+\phi_1(x_1)-\lambda(u_2-m_2-\phi_2(x_2))-\mu(x_1+x_2-y_j)-\eta(m_1+m_2+c_j(y_j)-\omega)
$$

FOC:
$$
\begin{cases}
\dfrac{\partial\mathcal{L}}{\partial m_1}=1-\eta=0 \\
\dfrac{\partial\mathcal{L}}{\partial m_2}=\lambda-\eta=0 \\
\dfrac{\partial\mathcal{L}}{\partial x_1}=\phi_1'(x_1)-\mu=0 \\
\dfrac{\partial\mathcal{L}}{\partial x_2}=\phi_2'(x_2)-\mu=0 \\
\dfrac{\partial\mathcal{L}}{\partial y_i}=\mu-\eta c_j'(y_j)=0 \\
\dfrac{\partial\mathcal{L}}{\partial \mu}=x_1+x_2-y_j=0 \quad\text{interior solution}
\end{cases}
\implies
\begin{cases}
1=\eta \\
\lambda=\eta \\
\phi_1'(x_1)=\mu \\
\phi_2'(x_2)=\mu \\
\mu=\eta c_j'(y_j) \\
x_1+x_2=y_j
\end{cases}\implies
\begin{cases}
\phi_1'(x_1)=\phi_2'(x_2)=c_j'(y_j) \\
x_1+x_2=y_j
\end{cases}
$$

### 2(b)

$$
\max_{
\begin{align}
m_1,x_1 \\
m_2,x_2
\end{align}
}
\quad W(u_1,u_2)\quad\textrm{s.t.}\quad
\begin{cases}
x_1+x_2\leq y_j & (\mu) \\
m_1+m_2+c_j(y_j)\leq\omega & (\eta) 
\end{cases}
$$

$$
\begin{cases}
u_1=m_1+\phi_1(x_1) \\
u_2=m_2+\phi_2(x_2)
\end{cases}
\implies W(m_1+\phi_1(x_1), m_2+\phi_2(x_2))
$$

$$
\mathcal{L}=W(m_1+\phi_1(x_1), m_2+\phi_2(x_2))-\mu(x_1+x_2-y_j)-\eta(m_1+m_2+c_j(y_j)-\omega)
$$

FOC:
$$
\begin{align}
(m_1):\quad & \frac{\partial\mathcal{L}}{\partial m_1}=\frac{\partial W}{\partial u_1}-\eta=0 \\
(m_2):\quad & \frac{\partial\mathcal{L}}{\partial m_2}=\frac{\partial W}{\partial u_2}-\eta=0 \\
(x_1):\quad & \frac{\partial\mathcal{L}}{\partial x_1}=\frac{\partial W}{\partial u_1}\phi_1'(x_1)-\mu=0 \\
(x_2):\quad & \frac{\partial\mathcal{L}}{\partial x_2}=\frac{\partial W}{\partial u_2}\phi_2'(x_2)-\mu=0 \\
(y_j):\quad & \frac{\partial\mathcal{L}}{\partial y_j}=\mu-\eta c_j'(y_j)=0 \\
(\mu):\quad & x_1+x_2-y_j=0
\end{align}
$$

$$
\begin{cases}
\dfrac{\partial W}{\partial u_1}-\eta=0 \\
\dfrac{\partial W}{\partial u_2}-\eta=0
\end{cases}
\implies
\frac{\partial W}{\partial u_1}=\frac{\partial W}{\partial u_2}
$$

$$
\begin{cases}
\dfrac{\partial W}{\partial u_1}\phi_1'(x_1)-\mu=0 \\
\dfrac{\partial W}{\partial u_2}\phi_2'(x_2)-\mu=0
\end{cases}
\implies
\frac{\partial W}{\partial u_1}\phi_1'(x_1)=\frac{\partial W}{\partial u_2}\phi_2'(x_2)
\implies \phi_1'(x_1)=\phi_2'(x_2)
$$

$$
c_j'(y_j)=\frac{\mu}{\eta}=\phi_1'(x_1)=\phi_2'(x_2)
$$

The optimal allocation is a Pareto optimum.



## 3. Partial Equilibrium: Unconditional Basic Income

* There are $I>1$ consumers with utility $u_i=m_i+\alpha_i\ln x_i$ , where $\alpha_i>0$ is a parameter.
* Each consumer holds one unit of the numeraire $(\omega_i=1)$ .
* There is a single firm with cost function $C(y)=y^2$ .
* $p>0$ denotes the price of consumption good.
* The firm raises a revenue $py$ .
* Total tax income is $T=\tau py, \tau\in[0,1]$ .
* Each consumer receives an income $\frac{T}{I}$ .

### 3(a)

**Consumer problem:**
$$
\begin{align}
\max_{x_i,m_i}\quad & m_i+\alpha_i\ln x_i \\
\textrm{s.t.}\quad & m_i+p\cdot x_i\leq\omega_i+\theta_i\Pi+\frac{T}{I}
\end{align}
$$

$$
\mathcal{L}=m_i+\alpha_i\ln x_i-\lambda(m_i+p\cdot x_i-1-\theta_i\Pi-\frac{T}{I}) 
$$

FOC:
$$
\begin{align}
\frac{\partial\mathcal{L}}{\partial m_i}&=1-\lambda=0 \implies \lambda=1 \\
\frac{\partial\mathcal{L}}{\partial x_i}&=\frac{\alpha_i}{x_i}-\lambda p=0 \implies x_i=\frac{\alpha_i}{p}

\end{align}
$$
**Firm problem:**
$$
\max_{y}\quad py-C(y)-T 
$$

$$
\mathcal{L}=(1-\tau)py-y^2
$$

$$
\frac{\partial\mathcal{L}}{\partial y}=(1-\tau)p-2y=0\implies y=\frac{1}{2}(1-\tau)p
$$

**Market clearing:**
$$
\begin{align}
y&=\sum_{i=1}^{I}x_i \\
\frac{1}{2}(1-\tau)p&=\frac{\sum_{i=1}^{I}\alpha_i}{p} \\
p^2&=\frac{2\sum_{i=1}^{I}\alpha_i}{1-\tau} \\
p^*&=\sqrt{\frac{2\sum_{i=1}^{I}\alpha_i}{1-\tau}}
\end{align}
$$

$$
x_i^*=\frac{\alpha_i}{p^*}=\alpha_i\sqrt{\frac{1-\tau}{2\sum_{i=1}^I\alpha_i}}
$$

$$
y^*=\frac{1}{2}(1-\tau)p^*=\sqrt{\frac{1-\tau}{2}\sum_{i=1}^I\alpha_i}
$$

$$
\begin{align}
\Pi^*&=(1-\tau)p^*y^*-(y^*)^2 \\
&=(1-\tau)\sqrt{\frac{2\sum_{i=1}^{I}\alpha_i}{1-\tau}}
\sqrt{\frac{1-\tau}{2}\sum_{i=1}^I\alpha_i}-\frac{1-\tau}{2}\sum_{i=1}^I\alpha_i \\
&=\frac{1-\tau}{2}\sum_{i=1}^I\alpha_i
\end{align}
$$

$$
T^*=\tau py=\tau\sum_{i=1}^I\alpha_i
$$

### 3(b)

$$
\begin{align}
x_i(\tau): \quad & \text{equilibrium consumption of consumer $i$} \\
X(\tau): \quad & \text{aggregate consumption} \\
s_i^*(\tau)=\frac{x_i(\tau)}{X(\tau)}:\quad & \text{relative consumption inequality} \\
x_i(\tau)-x_{i'}(\tau): \quad & \text{absolute consumption inequality}
\end{align}
$$

In equilibrium, we have
$$
x_i(\tau)=\alpha_i\sqrt{\frac{1-\tau}{2\sum_i\alpha_i}}
$$

$$
X(\tau)=\sum_ix_i(\tau)=\sum_i\alpha_i\sqrt{\frac{1-\tau}{2\sum_i\alpha_i}}
$$

Relative consumption inequality
$$
s_i^*(\tau)=\frac{x_i(\tau)}{X(\tau)}=\frac{\alpha_i}{\sum_i\alpha_i}\quad\text{indepedent of $\tau$}
$$
Absolute consumption inequality
$$
x_i(\tau)-x_{i'}(\tau)=(\alpha_i-\alpha_{i'})\sqrt{\frac{1-\tau}{2\sum_i\alpha_i}}
\quad\text{decreasing in $\tau$ if $\alpha_i>\alpha_{i'}$}
$$
**Explanation:** 

Price increase due to a higher tax leads to less consumption and more so for consumption intense consumers while relative consumption levels remain the same.

### 3(c)

$$
\text{Equilibrium income:}\quad w_i(\tau)=1+\theta_i\Pi+\frac{T}{I}\quad\text{where $\theta\in[0,1]$}
$$

$$
\begin{align}
w_i(\tau)&=1+\theta_i\Pi+\frac{T}{I} \\
&=1+\theta_i\frac{1-\tau}{2}\sum_{i=1}^I\alpha_i+\frac{\tau}{I}\sum_{i=1}^I\alpha_i \\
&=1+\frac{1}{2}\theta_i\sum_{i=1}^{I}\alpha_i+\tau\sum_{i=1}^{I}\alpha_i\left(\frac{1}{I}-\frac{\theta_i}{2} \right)
\end{align}
$$

**Absolute income inequality:**
$$
w_i(\tau)-w_{i'}(\tau)=\frac{1}{2}(\theta_i-\theta_{i'})\sum_{i=1}^{I}\alpha_i-
\frac{\tau}{2}(\theta_i-\theta_{i'})\sum_{i=1}^{I}\alpha_i=
\frac{1-\tau}{2}(\theta_i-\theta_{i'})\sum_{i=1}^{I}\alpha_i
$$
**Relative income inequality:**
$$
\begin{align}
\sum_{i=1}^{I}w_i(\tau)&=\sum_{i=1}^{I}
\left(1+\theta_i\frac{1-\tau}{2}\sum_{i=1}^I\alpha_i+\frac{\tau}{I}\sum_{i=1}^I\alpha_i \right) \\
&=I+\frac{1-\tau}{2}\sum_{i=1}^I\alpha_i+\tau\sum_{i=1}^I\alpha_i \\
&=I+\frac{1+\tau}{2}\sum_{i=1}^I\alpha_i\quad\text{increasing in $\tau$}
\end{align}
$$

$$
w_i(\tau)=1+\theta_i\frac{1-\tau}{2}\sum_{i=1}^I\alpha_i+\frac{\tau}{I}\sum_{i=1}^I\alpha_i 
\quad\text{can be decreasing in $\tau$ for high $\theta_i$}
$$

$$
\frac{w_i(\tau)}{\sum_{i=1}^{I}w_i(\tau)}\quad\text{decreasing in $\tau$ for high $\theta_i$}
$$

$$
\text{less income inequality in relative terms (depending on firm share $\theta_i$)}
$$

Do all consumers benefit?
$$
\begin{align}
m_i&=\omega_i+\theta_i\Pi+\frac{T}{I}-p\cdot x_i \\
&=1+\theta_i\frac{1-\tau}{2}\sum_{i=1}^I\alpha_i+\frac{\tau}{I}\sum_{i=1}^I\alpha_i-\sum_{i=1}^I\alpha_i \\
&=1+\left(\theta_i\frac{1-\tau}{2}+\frac{\tau}{I}-1\right)\sum_{i=1}^I\alpha_i
\end{align}
$$

$$
\begin{align}
u_i&=m_i+\alpha_i\ln(x_i) \\
&=1+\left(\theta_i\frac{1-\tau}{2}+\frac{\tau}{I}-1\right)\sum_{i=1}^I\alpha_i+\alpha_i
\ln\left(\alpha_i\sqrt{\frac{1-\tau}{2\sum_i\alpha_i}}\right)
\end{align}
$$

$$
\frac{\partial u_i}{\partial\tau}=\left(\frac{1}{I}-\frac{\theta_i}{2}\right)\sum_{i=1}^I\alpha_i-
\frac{\alpha_i}{2(1-\tau)}
$$

$$
\frac{\partial u_i}{\partial\tau}=
\underbrace{\left(\frac{1}{I}-\frac{\theta_i}{2}\right)\sum_{i=1}^I\alpha_i}_{\Delta W}-
\frac{\alpha_i}{2(1-\tau)}
$$

Income can decrease for high $\theta_1$-types. Not everyone benefits from unconditional basic income.

### (d)

$$
\begin{align}
U=\sum_{i=1}^{I}u_i&=I+\left(\frac{1-\tau}{2}+\tau-I \right)\sum_{i=1}^{I}\alpha_i+
\sum_{i=1}^{I}\alpha_i\ln\left(\alpha_i\sqrt{\frac{1-\tau}{2\sum_i\alpha_i}}\right) \\
&=I+\left(\frac{1+\tau}{2}-I \right)\sum_{i=1}^{I}\alpha_i+
\sum_{i=1}^{I}\alpha_i\ln\left(\alpha_i\sqrt{\frac{1-\tau}{2\sum_i\alpha_i}}\right)
\end{align}
$$

$$
\begin{align}
\frac{\partial U}{\partial\tau}&=\frac{1}{2}\sum_{i=1}^{I}\alpha_i+\frac{1}{2(1-\tau)}\sum_{i=1}^{I}\alpha_i \\
&=\left(\frac{1}{2}-\frac{1}{2(1-\tau)} \right)\sum_{i=1}^{I}\alpha_i\quad\text{Total welfare decreases in $\tau$}
\end{align}
$$

**Reason:**

Higher price due to higher tax leads to lower consumption of all consumers which dominates the income effect.

